\documentclass{article}
\usepackage[utf8]{inputenc}

\usepackage{amsmath}
\usepackage{amssymb}

\newcommand{\R}{\mathbb{R}}

\title{robotics1, HW 1}
\author{Aybek Bekbayev, 3462098, BSc Mathematik }
\date{April 2021}

\begin{document}

\maketitle

\section{Matrix equations (4 points)}

\paragraph{a)}
\text{Let $X$, $A$ be arbitrary matrices, A invertible. Solve for X:}
    \begin{center}
        $$
            XA + A^{T} = \textbf{I} 
        $$
        $$   
            A^{T}X^{T}+A = \textbf{I}^{T} = \textbf{I} 
        $$    
        $$
            X^T = (A^{-1})^{T}(\textbf{I}-A) 
        $$
        $$
            X = (\textbf{I} - A^{T})A^{-1}
        $$ 
    \end{center}
\paragraph{b)}
\text{ Let $X$, $A$, $B$ be arbitrary matrices, $(C - 2A^{T})$ invertible. Solve for X:}
\begin{center}
    $$
        X^{T}C=[2A(X+B)]^{T}
    $$
    $$
        X^{T}C = 2(X^{T} + B^{T})A^{T}  
    $$
    $$
        X^{T}C = 2X^{T}A^{T} + 2B^{T}A^{T}
    $$
    $$
        X^{T}(C-2A^{T}) = 2B^{T}A^{T}
    $$
    $$
        X^{T} = (C-2A^{T})^{-1}(2AB)^T
    $$
    $$
        X = 2AB((C-2A^{T})^{-1})^{T}
    $$
\end{center}
\paragraph{c)}
\begin{center}
    $$
        (Ax-y)^{T}A = \textbf{0}_{n}^{T}
    $$    
    $$
        x^{T}A^{T}A-y^{T}A = \textbf{0}^{T}_{n}
    $$
    $$
        x^{T}A^{T}A = y^{T}A
    $$
    $$
        A^{T}Ax = A^{T}y
    $$
    $$
        x = (A^{T}A)^{-1}A^{T}y
    $$
\end{center}
\paragraph{d)}
\begin{center}

\end{center}
\section{ Vector derivatives (5 points)}
Let $x$ \in \R$^{n}$, $y$ \in \R$^{d}$, $f$, $g$ : \R$^{n}$ \rightarrow \R$^{d}$, $A$ \in \R$^{n \times d}$, $C$ \in \R$^{d \times d}$. (Also provide the dimensionality of the results.) \\
a) What is $\frac{\partial}{\partial x}x$ ?
\begin{center}
    $\frac{\partial}{\partial x}x = \textbf{1}_{n}^{T}$ (shape is ($1$, $n$))
\end{center}
b) What is $\frac{\partial}{\partial x}x^Tx $
\begin{center}
    $\frac{\partial}{\partial x}x^Tx = 2x^{T}$ (shape is ($1$, $n$))
\end{center}
c) What is $\frac{\partial}{\partial x}[f(x)^Tf(x)]$
\begin{center}
    $\frac{\partial}{\partial x}[f(x)^{T}f(x)] = 2f(x)^{T}f^{'}(x)$\\
    $f(x)$ is shape of (d, 1) \\
    $f^{'}(x)$ is shape of (d, n) \\
    $f(x)^{T}f^{'}(x)$ is shape of (1, n)
    
\end{center}
d) What is $\frac{\partial}{\partial x}[f(x)^TCg(x)]$
\begin{center}
    $\frac{\partial}{\partial x}[f(x)^TCg(x)] = f(x)^{T}Cg^{'}(x) + g(x)^{T}C^{T}f^{'}(x)$ \\
    $f^{'}(x)$ and $g^{'}(x)$ are shape of $(d, n)$ \\
    $f(x)^{T}C$ is $(1, d) \times (d, d) = (1, d)$ \\
    $g(x)^{T}C^{T}$ is $(1, d) \times (d, d) = (1,d)$ \\
    $(1,d) \times (d, n) = (1, n)$ \\
    Shape of the derivative is $(1, n)$
\end{center}
e)
\begin{center}
    $$
        f(x) = (Ax-y)^{T}(Ax-y)+x^{T}Bx^{T}
    $$
    $$
        f^{'}(x) = 2(Ax-y)^{T}A + 2x^{T}B
    $$
    $$
        f^{'}(x) = 0
    $$
    $$
        2(Ax-y)^{T}A + 2x^{T}B = 0
    $$
    $$
        x^{T}A^{T}A-y^TA + x^{T}B = 0
    $$
    $$
        x^{T}(A^{T}A+B) = y^{T}A
    $$
    $$
        x = (A^TA+B^T)^{-1}A^{T}y
    $$
   
\end{center}
\end{document}
